Prove feval and fhas_type equivalent to the semantics

Stlc_fun.v
@@ -38,6 +38,7 @@ Qed.
 (******************************************************************************)
 (* has_type                                                                   *)
 (******************************************************************************)
+Print has_type.
 
 Fixpoint fhas_type (c : context) (e : expr) : option type :=
   match e with
@@ -54,6 +55,11 @@ Fixpoint fhas_type (c : context) (e : expr) : option type :=
           | None => None
           end
       | Some _ => None
+      | None => None
+      end
+  | elet x e1 e2 =>
+      match fhas_type c e1 with
+      | Some t1 => fhas_type (Context.add x t1 c) e2
       | None => None
       end
   end.
@@ -75,6 +81,9 @@ Proof.
     rewrite IHHAS_TYPE2.
     rewrite type_beq_refl.
     reflexivity.
+  - simpl.
+    rewrite IHHAS_TYPE1.
+    assumption.
 Qed.
 
 Theorem has_type_if_fhas_type : forall c e t,
@@ -107,6 +116,11 @@ Proof.
         }
         { discriminate. }
     + discriminate.
+  - inversion H; clear H.
+    destruct (fhas_type c e1) eqn:Heqn1; try discriminate.
+    destruct (fhas_type (Context.add v t c) e2) eqn:Heqn2; try discriminate.
+    inversion H1; subst.
+    eauto using has_type_let.
 Qed.
 
 Theorem has_type_iff_fhas_type : forall c e t,
@@ -136,43 +150,61 @@ Proof.
   - induction e; auto using value; inversion H.
 Qed.
 
+Theorem not_value_iff_is_value_false : forall e,
+  ~ value e <-> is_value e = false.
+Proof.
+Admitted.
+
 (******************************************************************************)
 (* feval                                                                      *)
 (******************************************************************************)
 
-Fixpoint feval (e : expr) : option expr :=
+Print eval.
+
+Fixpoint feval (h : heap) (e : expr) : option expr :=
   match e with
+  | eunit => None
+  | evar x => Heap.find x h
+  | eabs _ _ _ => None
   | eapp (eabs x t e) e2 =>
       if is_value e2 then
         Some (subst x e2 e)
       else
-        match feval e2 with
+        match feval h e2 with
         | Some v2 => Some (eapp (eabs x t e) v2)
         | None => None
         end
   | eapp e1 e2 =>
-      match feval e1 with
+      match feval h e1 with
       | Some v1 => Some (eapp v1 e2)
       | None => None
       end
-  | _ => None
+  | elet x e1 e2 =>
+      if is_value e1 then
+        Some (subst x e1 e2)
+      else
+        match feval h e1 with
+        | Some v1 => Some (elet x v1 e2)
+        | None => None
+        end
   end.
 
-Lemma not_value_if_eval : forall e1 e2, eval e1 e2 -> ~ value e1.
+Lemma not_value_if_eval : forall h e1 e2, eval h e1 e2 -> ~ value e1.
 Proof.
-  intros e1 e2 H.
-  inversion H; rewrite value_iff_is_value; discriminate.
+  intros h e1 e2 H.
+  inversion H; rewrite value_iff_is_value; try discriminate.
 Qed.
 
-Theorem feval_if_eval : forall c e1 e2 t,
+Theorem feval_if_eval : forall c h e1 e2 t,
   has_type c e1 t ->
-  eval e1 e2 ->
-  feval e1 = Some e2.
+  eval h e1 e2 ->
+  feval h e1 = Some e2.
 Proof.
-  intros c e1 e2 t HAS_TYPE EVAL.
+  intros c h e1 e2 t HAS_TYPE EVAL.
   generalize dependent t.
   generalize dependent c.
   induction EVAL; intros c ty HAS_TYPE.
+  - assumption.
   - simpl.
     destruct e1;
       inversion EVAL; inversion HAS_TYPE; subst;
@@ -189,48 +221,94 @@ Proof.
       rewrite EVAL.
       erewrite IHEVAL; eauto.
     + inversion H.
+    + inversion H.
   - apply value_iff_is_value in H.
     simpl.
     rewrite H.
     reflexivity.
+  - simpl.
+    inversion HAS_TYPE; clear HAS_TYPE; subst.
+    apply not_value_if_eval in EVAL.
+    rewrite value_iff_is_value in EVAL.
+    apply not_true_is_false in EVAL.
+    destruct (is_value e1) eqn:Heqn.
+    + discriminate.
+    + erewrite IHEVAL; eauto 1.
+  - simpl.
+    apply value_iff_is_value in H.
+    rewrite H.
+    reflexivity.
 Qed.
 
-Theorem eval_if_feval : forall c e1 e2 t,
-  has_type c e1 t ->
-  feval e1 = Some e2 ->
-  eval e1 e2.
+Lemma eval_if_not_value : forall e1,
+  ~ value e1 -> exists h e2, eval h e1 e2.
 Proof.
-  intros c e1.
+Admitted.
+
+Theorem eval_if_feval : forall c h e1 e2 t,
+  has_type c e1 t ->
+  feval h e1 = Some e2 ->
+  eval h e1 e2.
+Proof.
+  intros c h e1.
+  generalize dependent h.
   generalize dependent c.
-  induction e1; intros c e2 ty HAS_TYPE H.
+  induction e1; intros c h e2 ty HAS_TYPE H.
   - inversion H.
-  - inversion H.
+  - simpl in H.
+    apply eval_var.
+    assumption.
   - inversion H.
   - inversion HAS_TYPE; clear HAS_TYPE; subst.
     destruct e1_1 eqn:Heqn.
     + discriminate.
-    + discriminate.
+    + simpl in H.
+      destruct (Heap.find (elt:=expr) v h) eqn:Heqn2.
+      * inversion H.
+        apply eval_app1.
+        apply eval_var.
+        assumption.
+      * discriminate.
     + simpl in H.
       destruct (is_value e1_2) eqn:Heqn2.
       * inversion H.
         apply eval_beta.
         apply value_iff_is_value.
         assumption.
-      * destruct (feval e1_2);inversion H;
+      * destruct (feval h e1_2) eqn:Heqn3;
+          inversion H; clear H; subst;
           eauto using eval_app2, vabs.
     + rewrite <- Heqn in *.
       simpl in H.
-      destruct (feval e1_1) eqn:Heqn2.
+      destruct (feval h e1_1) eqn:Heqn2.
       * rewrite Heqn in *.
         inversion H.
         eauto using eval_app1.
       * rewrite Heqn in *.
         discriminate.
+    + rewrite <- Heqn in *.
+      simpl in H.
+      destruct (feval h e1_1) eqn:Heqn2.
+      * rewrite Heqn in *.
+        inversion H.
+        eauto using eval_app1.
+      * rewrite Heqn in *.
+        discriminate.
+  - inversion HAS_TYPE; clear HAS_TYPE; subst.
+    simpl in H.
+    destruct (is_value e1_1) eqn:Heqn1.
+    + inversion H; clear H; subst.
+      apply eval_let2.
+      apply value_iff_is_value.
+      assumption.
+    + destruct (feval h e1_1) eqn:Heqn2;
+        inversion H; clear H; subst;
+        eauto using eval_let1.
 Qed.
 
-Theorem eval_iff_feval : forall c e1 e2 t,
+Theorem eval_iff_feval : forall c h e1 e2 t,
   has_type c e1 t ->
-  eval e1 e2 <-> feval e1 = Some e2.
+  eval h e1 e2 <-> feval h e1 = Some e2.
 Proof.
   intros. split.
   - eauto 2 using feval_if_eval.
